set up type translation proof

rocq/rec/simple_equiv.v
@@ -217,6 +217,9 @@ Proof.
     econstructor; eauto with rec.
 Qed.
 
+(** * Program contexts *)
+
+
 
 (** * Nat-based equivalence and approximation *)
 
@@ -525,6 +528,312 @@ split.
 - intros. inversion H. eapply typed1; eauto.
 - intros. inversion H. eapply typed2; eauto.
 Qed.
+
+
+(** ------------------------------------------------- *)
+
+(*
+Variant ContextType : Type := TmCtx | ValCtx.
+Definition CT (T : ContextType) : nat -> Type := 
+  match T with | TmCtx => Tm | ValCtx => Val end.
+
+(* A context has two natural number indices. The first is the scope of the
+  hole, the second is the scope of the plugged term or value. (See definition
+  of plug below.)
+
+  A context also has two 'ContextType' indices. The first is the type of the
+  hole. Do we plug terms or values in to this Context. The second describes
+  whether this Context produces a term or value. For the second, we could
+  split the Context type in to TmContext and ValContext. However, when we talk
+  about composing contexts it is useful to be able to abstract over this
+  index.  
+*)
+Inductive Context (m : nat) : nat -> ContextType -> ContextType -> Type :=
+  | c_hole {T}    : Context m m T T
+  | c_app1 {n T}  : Context m n T ValCtx -> Val n -> Context m n T TmCtx
+  | c_app2 {n T}  : Val n -> Context m n T ValCtx -> Context m n T TmCtx
+  | c_let1 {n T}  : Context m n T TmCtx -> Tm (S n) -> Context m n T TmCtx
+  | c_let2 {n T}  : Tm n -> Context m (S n) T TmCtx -> Context m n T TmCtx
+  | c_ifz1 {n T}  : Context m n T ValCtx -> Tm n -> Tm (S n) -> Context m n T TmCtx
+  | c_ifz2 {n T}  : Val n -> Context m n T TmCtx -> Tm (S n) -> Context m n T TmCtx
+  | c_ifz3 {n T}  : Val n -> Tm n -> Context m (S n) T TmCtx -> Context m n T TmCtx
+  | c_ret  {n T}  : Context m n T ValCtx -> Context m n T TmCtx
+  | v_abs {n T}   : Context m (S n) T TmCtx -> Context m n T ValCtx
+  | v_succ {n T}  : Context m n T ValCtx -> Context m n T ValCtx
+.
+
+Arguments c_hole {_}{_}.
+Arguments c_app1 {_}{_}{_}.
+Arguments c_app2 {_}{_}{_}.
+Arguments c_let1 {_}{_}{_}.
+Arguments c_let2 {_}{_}{_}.
+Arguments c_ifz1 {_}{_}{_}.
+Arguments c_ifz2 {_}{_}{_}.
+Arguments c_ifz3 {_}{_}{_}.
+Arguments c_ret {_}{_}{_}.
+Arguments v_abs {_}{_}{_}.
+Arguments v_succ {_}{_}{_}.
+
+Local Notation "#" := c_hole (at level 7).
+
+(* Do this in interactive mode to make working with the dependent types
+   easier. But don't automate too much to make sure that we get the 
+   arguments in the right order in app/case/prod *)
+Fixpoint plug {m}{n}{T1 T2 : ContextType} (C : Context m n T1 T2) : CT T1 m -> CT T2 n.
+destruct C.
+all: intros e.
+- eapply e.
+- eapply (app (plug _ _ _ _ C e) v). 
+- eapply (app v (plug _ _ _ _ C e)).
+- eapply (let_ (plug _ _ _ _ C e) t).
+- eapply (let_ t (plug _ _ _ _ C e)).
+- eapply (ifz (plug _ _ _ _ C e) t t0).
+- eapply (ifz v (plug _ _ _ _ C e) t).
+- eapply (ifz v t (plug _ _ _ _ C e)).
+- eapply (ret (plug _ _ _ _ C e)).
+- eapply (abs (plug _ _ _ _ C e)).
+- eapply (succ (plug _ _ _ _ C e)).
+Defined.
+
+Notation "C {| e |} " := (plug C e). 
+
+Fixpoint compose {m n p}{T1 T2 T3} (C1 : Context m n T1 T2) (C2 : Context n p T2 T3) : Context m p T1 T3.
+- dependent destruction C2.
+  + exact C1.
+  + eapply c_app1; eauto.
+  + eapply c_app2; eauto.
+  + eapply c_let1; eauto.
+  + eapply c_let2; eauto.
+  + eapply c_ifz1; eauto.
+  + eapply c_ifz2; eauto.
+  + eapply c_ifz3; eauto.
+  + eapply c_ret; eauto.
+  + eapply v_abs; eauto.
+  + eapply v_succ; eauto.
+Defined.
+
+Infix "∘" := compose (at level 70).
+
+Fixpoint compose_plug  {m n p T1 T2 T3} (C1 : Context m n T1 T2) (C2 : Context n p T2 T3) e : 
+  C2 {| C1 {| e |} |} = (C1 ∘ C2) {| e |}.
+Proof.
+  dependent destruction C2.
+  all: cbn.
+  all: try (rewrite compose_plug; done).
+  done.
+Qed.
+
+Reserved Notation "C ∈C Γ ▷ τ ⤳ Δ ▷ τ'" (at level 70).
+
+Inductive typing_Context m (Γ : Ctx m) (τ : Ty 0) : forall n (Δ : Ctx n) (τ' : Ty 0) T1 T2, Context m n T1 T2 -> Prop :=
+  | ctx_hole T : (@c_hole _ T) ∈C Γ ▷ τ ⤳ Γ ▷ τ
+  | ctx_app1 m (Δ : Ctx m) τ1 τ2  T1 C v : 
+    (C ∈C Γ ▷ τ ⤳ Δ ▷ Arr τ1 τ2) ->
+    (Δ |-v v ∈ τ1) ->
+    (@c_app1 _ _ T1 C v) ∈C Γ ▷ τ ⤳ Δ ▷ τ2
+ | ctx_app2  m (Δ : Ctx m) τ1 τ2  T1 C v : 
+    (Δ |-v v ∈ Arr τ1 τ2) ->
+    (C ∈C Γ ▷ τ ⤳ Δ ▷ τ1) ->
+    (@c_app2 _ _ T1 v C) ∈C Γ ▷ τ ⤳ Δ ▷ τ2
+ | ctx_let1  m (Δ : Ctx m) τ1 τ2  T1 C e : 
+    (C ∈C Γ ▷ τ ⤳ Δ ▷ τ1) ->
+    (τ1 .: Δ |-e e ∈ τ2) ->
+    (@c_let1 _ _ T1 C e) ∈C Γ ▷ τ ⤳ Δ ▷ τ2
+ | ctx_let2  m (Δ : Ctx m) τ1 τ2  T1 C e : 
+    (Δ |-e e ∈ τ1) ->
+    (C ∈C  Γ ▷ τ ⤳ τ1 .: Δ ▷ τ2) ->
+    (@c_let2 _ _ T1 e C) ∈C Γ ▷ τ ⤳ Δ ▷ τ2
+ | ctx_ret   m (Δ : Ctx m) τ1 T1 C : 
+    (C ∈C Γ ▷ τ ⤳ Δ ▷ τ1) -> 
+    (@c_ret _ _ T1 C) ∈C Γ ▷ τ ⤳ Δ ▷ τ1
+ | ctx_abs   m (Δ : Ctx m) τ1 τ2 T1 C : 
+    (C ∈C Γ ▷ τ ⤳ τ1 .: Δ ▷ τ2) -> 
+    (@v_abs _ _ T1 C) ∈C Γ ▷ τ ⤳ Δ ▷ Arr τ1 τ2
+
+where 
+    "C ∈C Γ ▷ τ ⤳ Δ ▷ τ'" := (typing_Context _ Γ τ _ Δ τ' _ _ C).
+
+
+
+(** * "Contextual Equivalence" *)
+Definition Contextual (n : nat) Γ (e1 : Tm n) (e2 : Tm n) τ :=
+    Γ |-e e1 ∈ τ /\
+    Γ |-e e2 ∈ τ /\ 
+  forall (C :Context n 0 TmCtx TmCtx), 
+    C ∈C Γ ▷ τ ⤳ null ▷ Nat -> 
+       exists n, (nil, C {|e1|}) ↦* (nil, ret n) /\ (nil, C{|e2|}) ↦* (nil, ret n).
+Definition ContextualVal (n : nat) Γ (v1 : Val n) (v2 : Val n) τ := 
+  Γ |-v v1 ∈ τ /\
+  Γ |-v v2 ∈ τ /\ 
+  forall (C :Context n 0 ValCtx TmCtx), 
+    C ∈C Γ ▷ τ ⤳ null ▷ Nat -> 
+       exists n, (nil, C {|v1|}) ↦* (nil, ret n) /\ (nil, C{|v2|}) ↦* (nil, ret n).
+
+Instance Adequate_Contextual : Adequate Contextual.
+Proof.
+  unfold Adequate.
+  intros e e' C.
+  unfold Contextual in C.
+  move: C => [T1 [T2 C]].
+  specialize (C #).
+  cbn in C.
+  asimpl in C.
+Admitted.
+
+Lemma Transitive_Contextual : ScopedTransitive Contextual.
+Proof.
+  intros n e1 e2 e3 CT1 CT2 C h.
+  unfold Contextual in CT1, CT2.
+  eauto.
+Qed.
+
+(** If two terms are contextually related, then any larger terms from plugging 
+    them into a context are also related. *)
+Lemma Contextual_Replacement n e1 e2 : 
+  Contextual n e1 e2 -> 
+  forall m (C : Context n m TmCtx TmCtx), Contextual m (C{| e1 |}) (C{| e2|}).
+Proof.
+  intros h m C.
+  unfold Contextual in *.
+  intros C0. 
+  repeat rewrite compose_plug.
+  eapply h.
+Qed.
+
+Ltac compose_rewrite C1 := 
+  repeat rewrite <- compose_plug in C1; cbn in C1; asimpl in C1; auto.
+
+Instance Compatible_Contextual : Compatible Contextual ContextualVal.
+split.
+all: intros n.
+all: repeat unfold Contextual, ContextualVal.
+- intros x C. intro h. done.
+- intros C. done.
+- intros C. done.
+- (* succ *)
+  intros v1 v2 C1 C h.
+  specialize (@C1 (v_succ # ∘ C)).
+  compose_rewrite C1.
+
+- (* abs *)
+  intros e1 e2 C1 C h.
+  specialize (@C1 (v_abs # ∘ C)).
+  compose_rewrite C1.
+
+- (* ret *)
+  intros v1 v2 C1 C h.
+  specialize (@C1 (c_ret # ∘ C)).
+  compose_rewrite C1.
+- (* let *) 
+  intros e1 e2 e1' e2' C1 C2 C h.
+  specialize (@C2 (c_let2 e2 # ∘ C)).
+  compose_rewrite C2.
+  specialize (@C1 (c_let1 # e1' ∘ C)).
+  compose_rewrite C1.
+- (* ifz *)
+  intros v1 v2 e1 e2 e1' e2' C1 C2 C3 C h.
+  specialize (@C3 (c_ifz3 v1 e1 # ∘ C)).
+  compose_rewrite C3.
+  specialize (@C2 (c_ifz2 v1 # e2' ∘ C)).
+  compose_rewrite C2.
+  specialize (@C1 (c_ifz1 # e2 e2' ∘ C)).
+  compose_rewrite C1.
+
+- (* app *)
+  intros v1 v2 v1' v2' C1 C2 C.
+  specialize (@C2 (c_app2 v2 # ∘ C)).
+  compose_rewrite C2.
+  specialize (@C1 (c_app1 # v1' ∘ C)).
+  compose_rewrite C1.
+
+Qed.
+
+(** * Contextual equivalence implies CTX *)
+Lemma Contextual_CTX n e1 e2 : Contextual n e1 e2 -> CTX n e1 e2.
+Proof.
+  intro h. 
+  exists Contextual ContextualVal; eauto.
+  eapply Compatible_Contextual.
+  eapply Adequate_Contextual.
+  eapply Transitive_Contextual.
+Qed.
+
+
+(* ---------------------------------------------------- *)
+
+(** * If RE is a compatible relation and relates two terms, then it 
+      also related the terms in an arbitrary context *)
+Fixpoint Compatible_plug n (e1 e2 : Tm n) 
+  (RE : scoped_relation Tm)
+  (RV : scoped_relation Val)
+  (H : Compatible RE RV) :
+  RE n e1 e2 -> forall m (C : Context n m TmCtx TmCtx),
+  RE m C {|e1|} C {|e2|} 
+with 
+  Compatible_vplug n (e1 e2 : Tm n) 
+  (RE : scoped_relation Tm)
+  (RV : scoped_relation Val)
+  (H : Compatible RE RV) :
+  RE n e1 e2 -> forall m (C: Context n m TmCtx ValCtx),
+  RV m (C {|e1|}) (C{|e2|}).
+Proof.
+- intros h m C.
+  dependent destruction C.
+  all: cbn.
+  all: specialize (Compatible_plug n e1 e2 RE RV H h).
+  all: specialize (Compatible_vplug n e1 e2 RE RV H h).
+  + auto.
+  + eapply comp_app. 
+    eapply Compatible_vplug; eauto.
+    eapply scoped_refl. typeclasses eauto.
+  + eapply comp_app. eapply scoped_refl. typeclasses eauto.
+    eapply Compatible_vplug; eauto.
+  + eapply comp_let. eapply Compatible_plug; eauto.
+    eapply scoped_refl. typeclasses eauto.
+  + eapply comp_let. 
+    eapply scoped_refl. typeclasses eauto.
+    eapply Compatible_plug.
+  + eapply comp_ifz.
+    eapply Compatible_vplug.
+    eapply scoped_refl. typeclasses eauto.
+    eapply scoped_refl. typeclasses eauto.
+  + eapply comp_ifz.
+    eapply scoped_refl. typeclasses eauto.
+    eapply Compatible_plug.
+    eapply scoped_refl. typeclasses eauto.
+  + eapply comp_ifz.
+    eapply scoped_refl. typeclasses eauto.
+    eapply scoped_refl. typeclasses eauto.
+    eapply Compatible_plug.
+  + eapply comp_ret. 
+    eapply Compatible_vplug.
+
+- intros h m C.
+  dependent destruction C.
+  all: cbn.
+  all: specialize (Compatible_plug n e1 e2 RE RV H h).
+  all: specialize (Compatible_vplug n e1 e2 RE RV H h).
+  + eapply val_abs. eauto.
+  + eapply val_succ. eauto.
+
+Qed.
+
+(** * CTX implies Contextual *)
+Lemma CTX_Contextual n e1 e2 : 
+  CTX n e1 e2 -> Contextual n e1 e2.
+Proof.
+  intro h. 
+  unfold Contextual.
+  intros C.
+  destruct h.
+  eapply H0.
+  eapply Compatible_plug; eauto.
+Qed.
+
+*)
+
+
+
 
 (** ------------------------------------------------- *)
 
